---
layout: post
title:  "Review Cat Logic + Type Theory (Jacobs) §1.1"
date:   2023-12-17 00:56:11 -0400
categories: Type-Theory
---

Ref
1. https://people.mpi-sws.org/~dreyer/courses/catlogic/jacobs.pdf

***
Doing exercise for Ref1, § 1.1


***
# Recall Definitions (Ref1, 1.1.3)
let `p : 𝔼 → 𝔹` be a functor
1. `f : X → Y` is **carteisan over** `u : I → J` when
   1. `pf = u`, and
   2. for arbitrary `g : Z → Y`, `w : pZ → I` s.t. `pg = pf ∘ u`
   3. there exists a *unique* `h : Z → X` s.t. `ph = w` and `g = f ∘ h`
   4. Basically unique lifting for arbitrary factorization
2. `f` is cartesian if it cartsian over some arrow
3. functor `p` is fibration if 
   1. for every `Y ∈ 𝔼` and `u : I → pY`, there exists a cartesian morphism `f ∈ 𝔼` over `u`
4. (Ref1, P26) the fibre category `𝔼_I` is the category
   1. with objects `X ∈ 𝔼` s.t. pX = I
   2. with morpisms `f : X → Y ∈ 𝔼` s.t. `pf = id`
5. (Ref1, P26) Define for `u : pX → pY ∈ 𝔹`, `𝔼u := {f : X → Y| pf = u}`

***

* (Ref1, 1.1.4) : Cartesian lifting is unique
Given `f, f'` over `u`, we know `pf = pf' = u` thus `pf` and `pf'` factored each other  via `id`, i.e.
`pf ∘ id = pf' = pf = pf' ∘ id`，

Lift this 2 factorization, we get `f = f' ∘ h1`, `f' = f ∘ h2` with (†) two uniqueness property.

Thus `f = f ∘ h2 ∘ h1` and 
Since `f = f ∘ id` and `f' = f' ∘ id`, by (†), we can conclude `h2∘h1 = h1∘h2 = id`

* Exercise 1.1.1 (ii)
Since `p(f∘g)` and `p(f∘h)` both factors by `pf` by `pg = ph`, we have a unique `g = h` over `pg = ph`

* Exercise 1.1.2 **Alternative Definition!**
Let `p: 𝔼 → 𝔹`
f is Cartesian iff 
for arbitrary `Z ∈ 𝔼` and `w : pZ → pX`, 𝔼_{w}(Z, X) ---(f ∘ -)---> 𝔼_{u∘w}(Z, Y) is an isomorphism

The isomorphism comes from uniqueness.

The same graph in (Ref1, Def 1.1.3) is helpful. This definition is easier to remember



* Exercise 1.1.3
Given a fibration `p : 𝔼 → 𝔹`
1. every morphism factors `f : X → Y` as a vertical map followed by a cartesian one
Since `pf = pf ∘ id`, so we have a unique arrow `x` ,s.t. `px = id` with `f = f ∘ x`

* Exercise 1.1.3(2) 
we are actually proving something stronger
a cartesian map `f` over an isomorphism is an isomorphism
Note that we don't need fibration `p : 𝔼 → 𝔹`

Since we can factor `id` via `pf` as `pf` is an isomorphic, i.e. `p id = (pf)⁻¹ ∘ (pf)`, so there is a unique arrow
`x`, s.t. `f ∘ x = id`

What's more, we can factor `f` via `f`, i.e. `f ∘ id = f = f ∘ x ∘ f`, both `id` and `x ∘ f` are vertical map. By uniqueness of cartesian lifting, we canconclude `x ∘ f = id`

* Exercise 1.1.4, 
<!-- * For a fibration `p : 𝔼 → 𝔹` -->
1. All isomorphism in 𝔼 are Cartesian
Of course because all isomorphism `f : X → Y` can uniquely factor arbitrary `g : Z → Y`, i.e. `g = g ∘ f⁻₁ ∘ f` 
2. Composition of cartesian morphism is still cartesian
Trivial when using the alternative definition by 1.1.2
3. Trivial when using the alternative definition by 1.1.2.
4. Prove using 3. Since 3 tells us if `g∘f` and `g` are both cartesian, then `f` is cartesian. It is helpful when showing the existence of the cartesian lifting

* Exercise 1.1.5
* Exercise 1.1.6
(=>) We can prove
1. every strong cartesian lifting is a weak cartesian lifting
2. every weak cartesian lifting is unique up to iso
3. thus every weak cartesian lifting is also strong cartesian lifting 
   1. as each base morphism has a strong lifting, and its weak cartesian lifting is iso to that strong one, thus strong as well
4. thus composition of two weak(strong) cartesian lifting is also a weak(strong) cartesian lifting
(<=)

* Exercise 1.1.7
2 and 4 are trivial. Because X → I in 4 doesn't have arrows at all!
1 and 3 are just using definition

Recall the deifnition of fibration : for `p : 𝔼 → 𝔹`, for arbitrary `Y ∈ 𝔹` and `u : I → pY`, we have a cartesian morphism above `u`

* Exercise 1.1.8
1. trivial
2. Show `dom : 𝔹^→ → 𝔹` is a fibration
i.e. for arbitrary `(X' → X) ∈ 𝔹^→` and arbitrary `Y' → dom(X' → X) = Y' → X'`, we have ...

basically the graph is like 

Y' --f---> X' <--------Z'
|          |           |
g∘f        g           |
|          |           |
Y ---id---> X  <--------Z

Now we have an arrow Z' → Y', we need an arrow from Z → Y. Possible because `id : Y → X`

Why is it unique? still because that id

3. 